cleanup

history.fst
@@ -1,4 +1,5 @@
 module History
+
 open FStar.Tactics
 module T = FStar.Tactics
 open FStar.Tactics.Typeclasses
@@ -16,37 +17,6 @@ type history  =
             -> children:list (I.trace * history)
             -> history
 
-(*Returns true if h1 happens before h2*)
-val hb : h1:history -> h2:history -> Tot bool (decreases %[h1]) 
-val hb' : l:list (I.trace * history) -> s:state  -> h2:history -> Tot bool (decreases %[l])
-
-let rec hb h1 h2 =
-  let History s ch = h1 in 
-  hb' ch s h2 
-and hb' children par_state h2 =
-  match children with
-  | [] -> false
-  | (tr,x)::xs -> x = h2 ||
-                hb x h2 ||
-                hb' xs par_state h2
-  
-
-val eq : h1:history -> h2:history -> Tot bool (decreases %[h1]) 
-let eq h1 h2 = (h1 = h2)
-
-(*Returns true if h1 happens before or equal to h2*)
-val hbeq : h1:history -> h2:history -> Tot bool (decreases %[h1])
-let hbeq h1 h2 = hb h1 h2 || eq h1 h2
-
-val concurrent : h1:history -> h2:history -> Tot bool (decreases %[h1])
-let concurrent h1 h2 = not (hbeq h1 h2 || hbeq h2 h1)
-          
-val concurrent_commutative : h1:history
-                             -> h2:history{concurrent h1 h2}
-                             -> Lemma (ensures (concurrent h2 h1))
-let concurrent_commutative h1 h2 = ()
-
-
 val size : h:history -> Tot nat (decreases %[h])
 val size' : l:list (I.trace * history) -> Tot nat (decreases %[l])
 let rec size h =
@@ -57,43 +27,43 @@ and size'  l =
     | [] -> 0
     | (tr,x)::xs -> size x + size' xs
 
+val hb : h1:history -> h2:history -> Tot bool (decreases (size h1))
+let rec hb (History s ch) h2 = 
+  match ch with
+  | [] -> false
+  | (_,x)::xs -> x = h2 || hb x h2 || hb (History s xs) h2
 
-(*Returns true if all the children of a parent node are concurrent*)
-val concur_ch : l:list(I.trace * history) -> Tot bool (decreases %[l])
-val concur_ch' : child:history -> l:list(I.trace * history) -> Tot bool (decreases %[l])
-let rec concur_ch l = 
-match l with 
-  |[] -> true
-  |(tr,x)::xs -> concur_ch' x xs && concur_ch xs
-and concur_ch' x ch =
-match ch with
-  |[] -> true
-  |(tr,y)::xs -> concurrent x y && concur_ch' x xs
+(* h1 --hb--> h2 <==> hbeq h1 h2 = true *)
+val hbeq : h1:history -> h2:history -> bool
+let hbeq h1 h2 = h1 = h2 || hb h1 h2
 
+val concurrent : h1:history -> h2:history -> bool
+let concurrent h1 h2 = not (hb h1 h2 || hb h2 h1 || h1 = h2)
+
+val concurrent_commutative : h1:history
+                           -> h2:history{concurrent h1 h2}
+                           -> Lemma (ensures (concurrent h2 h1))
+let concurrent_commutative h1 h2 = ()
 
 val wellformed : h:history -> Tot bool (decreases h)
 val wellformed' : s:state -> l:list (I.trace * history) -> h:history -> Tot bool (decreases l)
 let rec wellformed h =
   let History state ch = h in
- (* concur_ch #n ch &&      //not necessary// *)
   wellformed' state ch h
 and wellformed' par_state children par_history =
   match children with
   | [] -> true
-  | (tr,ch_history)::xs -> 
-         let ch_state = History?.state ch_history in
-         hb par_history ch_history &&
-         ch_state = M.apply_tr par_state tr &&
-         wellformed ch_history &&
+  | (tr,x)::xs -> 
+         hb par_history x &&
+         M.apply_tr par_state tr = (History?.state x) &&
+         wellformed x &&
          wellformed' par_state xs par_history
-    
-
 
 let _ = assert (hbeq  (History 1 [([I.Inc 1;I.Inc 1], (History 3 [([I.Inc 1],(History 4 []))]))]) (History 3 [([I.Inc 1],(History 4 []))]));()
 
 let _ = assert (hb (History 1 [([I.Inc 1;I.Inc 1], (History 3 [([I.Inc 1],(History 4 []))]))]) (History 4 []));()
 
-let _ = assert (eq (History 1 [([I.Inc 1;I.Inc 1], (History 3 [([I.Inc 1],(History 4 []))]))]) (History 1 [([I.Inc 1;I.Inc 1], (History 3 [([I.Inc 1],(History 4 []))]))]));()
+let _ = assert ((History 1 [([I.Inc 1;I.Inc 1], (History 3 [([I.Inc 1],(History 4 []))]))])  = (History 1 [([I.Inc 1;I.Inc 1], (History 3 [([I.Inc 1],(History 4 []))]))]));()
 
 let _ = assert (wellformed (History 1 [([I.Inc 1;I.Inc 2], (History 4 [([I.Inc 1],(History 5 []))]))]));()
 
@@ -102,12 +72,11 @@ val hbeq_reflexive : h:history
                      -> Lemma (ensures (hbeq h h))
 let hbeq_reflexive h = ()
 
-
-
 val lemma1 : h:history {wellformed h}
-             -> Lemma (ensures (forall h'. hbeq h h' ==> wellformed h'))  (decreases (size h))
-                       
-let rec lemma1 (History s ch) = match ch with
- | [] -> ()
- | (tr,x)::xs -> lemma1 x; lemma1 (History s xs)
-          
+           -> Lemma (ensures (forall h'. hbeq h h' ==> wellformed h'))  (decreases (size h))
+let rec lemma1 (History s ch) = 
+  match ch with
+  | [] -> ()
+  | (_,x)::xs -> 
+     lemma1 x; 
+     lemma1 (History s xs)
